LeanNanoLlvm/Semantics/Denote.lean
@@ -9,6 +9,17 @@ open Std
 
 variable {φ : Nat}
 
+@[simp_wellform]
+def RegisterValue.WellFormedFor : AST.LlvmType φ → RegisterValue → Prop
+  | .int wTy, .bv wVal _ => wTy = wVal
+  | _, _ => False
+
+@[simp_wellform]
+def Definition.ArgValuesWellFormed (defn : @AST.Definition φ) (argVals : List RegisterValue) : Prop :=
+  match defn.prototype.type with
+  | .function _ argTys => List.Forall₂ RegisterValue.WellFormedFor argTys argVals
+  | _ => False
+
 @[simp_llvm]
 def denoteIntBinaryOp {w : Nat} (op : AST.IntBinaryOp) (x y : IntW w) : IntW w :=
   match op with
